\documentclass[preview]{standalone}
\usepackage[english]{babel}
\usepackage{amsmath}
\usepackage{amssymb}
\begin{document}
\begin{align*}
\vec{a} - \vec{b} = \vec{a} + - \vec{b} = \begin{bmatrix} \text{-}1 \\ 2 \end{bmatrix} + - \begin{bmatrix} 2 \\ 3 \end{bmatrix} = \begin{bmatrix} \text{-}1 \\ 2 \end{bmatrix} + \begin{bmatrix} \text{-}2 \\ \text{-}3 \end{bmatrix}= \begin{bmatrix} \text{-}1 + \text{-}2 \\ 2 + \text{-}3 \end{bmatrix} \begin{bmatrix} \text{-}3 \\ \text{-}1 \end{bmatrix}
\end{align*}
\end{document}